Manual/BasicTypes/Fin.lean
@@ -1,0 +1,296 @@
+/-
+Copyright (c) 2025 Lean FRO LLC. All rights reserved.
+Released under Apache 2.0 license as described in the file LICENSE.
+Author: David Thrane Christiansen
+-/
+
+import VersoManual
+
+import Manual.Meta
+
+open Manual.FFIDocType
+
+open Verso.Genre Manual
+
+#doc (Manual) "Finite Natural Numbers" =>
+%%%
+tag := "Fin"
+%%%
+
+```lean (show := false)
+section
+variable (n : Nat)
+```
+
+For any {tech}[natural number] {lean}`n`, the {lean}`Fin n` is a type that contains all the natural numbers that are strictly less than {lean}`n`.
+In other words, {lean}`Fin n` has exactly {lean}`n` elements.
+It can be used to represent the valid indices into a list or array, or it can serve as a canonical {lean}`n`-element type.
+
+{docstring Fin}
+
+{lean}`Fin` is closely related to {name}`UInt8`, {name}`UInt16`, {name}`UInt32`, {name}`UInt64`, and {name}`USize`, which also represent finite non-negative integral types.
+However, these types are backed by bitvectors rather than by natural numbers, and they have fixed bounds.
+{lean}`Fin` is comparatively more flexible, but also less convenient for low-level reasoning.
+In particular, using bitvectors rather than proofs that a number is less than some power of two avoids needing to take care to avoid evaluating the concrete bound.
+
+# Run-Time Characteristics
+
+Because {lean}`Fin n` is a structure in which only a single field is not a proof, it is a {ref "inductive-types-trivial-wrappers"}[trivial wrapper].
+This means that it is represented identically to the underlying natural number in compiled code.
+
+# Coercions and Literals
+
+There is a {tech}[coercion] from {lean}`Fin n` to {lean}`Nat` that discards the proof that the number is less than the bound.
+In particular, this coercion is precisely the projection {name}`Fin.val`.
+One consequence of this is that uses of {name}`Fin.val` are displayed as coercions rather than explicit projections in proof states.
+:::example "Coercing from {name}`Fin` to {name}`Nat`"
+A {lean}`Fin n` can be used where a {lean}`Nat` is expected:
+```lean (name := oneFinCoe)
+#eval let one : Fin 3 := ⟨1, by omega⟩; (one : Nat)
+```
+```leanOutput oneFinCoe
+1
+```
+
+Uses of {name}`Fin.val` show up as coercions in proof states:
+```proofState
+∀(n : Nat) (i : Fin n), i < n := by
+  intro n i
+/--
+n : Nat
+i : Fin n
+⊢ ↑i < n
+-/
+
+```
+:::
+
+Natural number literals may be used for {lean}`Fin` types, implemented as usual via an {name}`OfNat` instance.
+The {name}`OfNat` instance for {lean}`Fin n` requires that the upper bound {lean}`n` is not zero, but does not check that the literal is less than {lean}`n`.
+If the literal is larger than the type can represent, the remainder when dividing it by {lean}`n` is used.
+
+:::example "Numeric Literals for {name}`Fin`"
+
+If {lean}`n > 0`, then natural number literals can be used for {lean}`Fin n`:
+```lean
+example : Fin 5 := 3
+example : Fin 20 := 19
+```
+When the literal is greater than or equal to {lean}`n`, the remainder when dividing by {lean}`n` is used:
+```lean (name := fivethree)
+#eval (5 : Fin 3)
+```
+```leanOutput fivethree
+2
+```
+```lean (name := fourthree)
+#eval ([0, 1, 2, 3, 4, 5, 6] : List (Fin 3))
+```
+```leanOutput fourthree
+[0, 1, 2, 0, 1, 2, 0]
+```
+
+If Lean can't synthesize an instance of {lean}`NeZero n`, then there is no {lean}`OfNat (Fin n)` instance:
+```lean (error := true) (name := fin0)
+example : Fin 0 := 0
+```
+```leanOutput fin0
+failed to synthesize
+  OfNat (Fin 0) 0
+numerals are polymorphic in Lean, but the numeral `0` cannot be used in a context where the expected type is
+  Fin 0
+due to the absence of the instance above
+Additional diagnostic information may be available using the `set_option diagnostics true` command.
+```
+
+```lean (error := true) (name := finK)
+example (k : Nat) : Fin k := 0
+```
+```leanOutput finK
+failed to synthesize
+  OfNat (Fin k) 0
+numerals are polymorphic in Lean, but the numeral `0` cannot be used in a context where the expected type is
+  Fin k
+due to the absence of the instance above
+Additional diagnostic information may be available using the `set_option diagnostics true` command.
+```
+
+:::
+
+# API Reference
+
+## Construction
+
+{docstring Fin.last}
+
+{docstring Fin.succ}
+
+{docstring Fin.pred}
+
+## Arithmetic
+
+Typically, arithmetic operations on {name}`Fin` should be accessed using Lean's overloaded arithmetic notation, particularly via the instances {inst}`Add (Fin n)`, {inst}`Sub (Fin n)`, {inst}`Mul (Fin n)`, {inst}`Div (Fin n)`,  and {inst}`Mod (Fin n)`.
+Heterogeneous operators such as {lean}`Fin.natAdd` do not have corresponding heterogeneous instances (e.g. {name}`HAdd`) to avoid confusing type inference behavior.
+
+{docstring Fin.add}
+
+{docstring Fin.natAdd}
+
+{docstring Fin.addNat}
+
+{docstring Fin.mul}
+
+{docstring Fin.sub}
+
+{docstring Fin.subNat}
+
+{docstring Fin.div}
+
+{docstring Fin.mod}
+
+{docstring Fin.modn}
+
+{docstring Fin.log2}
+
+## Bitwise and Logical Operations
+
+Typically, bitwise and logical operations on {name}`Fin` should be accessed using Lean's overloaded arithmetic notation, particularly via the instances {inst}`ShiftLeft (Fin n)`, {inst}`ShiftRight (Fin n)`, {inst}`AndOp (Fin n)`, {inst}`OrOp (Fin n)`, {inst}`Xor (Fin n)`
+
+{docstring Fin.shiftLeft}
+
+{docstring Fin.shiftRight}
+
+{docstring Fin.land}
+
+{docstring Fin.lor}
+
+{docstring Fin.xor}
+
+
+## Conversions
+
+{docstring Fin.ofNat'}
+
+{docstring Fin.cast}
+
+{docstring Fin.castAdd}
+
+{docstring Fin.castLE}
+
+{docstring Fin.castSucc}
+
+{docstring Fin.castLT}
+
+{docstring Fin.rev}
+
+{docstring Fin.elim0}
+
+## Iteration
+
+{docstring Fin.foldr}
+
+{docstring Fin.foldrM}
+
+{docstring Fin.foldl}
+
+{docstring Fin.foldlM}
+
+{docstring Fin.hIterate}
+
+{docstring Fin.hIterateFrom}
+
+## Reasoning
+
+{docstring Fin.induction}
+
+{docstring Fin.inductionOn}
+
+{docstring Fin.reverseInduction}
+
+{docstring Fin.cases}
+
+{docstring Fin.lastCases}
+
+{docstring Fin.addCases}
+
+{docstring Fin.succRec}
+
+{docstring Fin.succRecOn}
+
+## Proof Automation
+
+{docstring Fin.isValue}
+
+{docstring Fin.fromExpr?}
+
+{docstring Fin.reduceOfNat'}
+
+{docstring Fin.reduceSucc}
+
+{docstring Fin.reduceAdd}
+
+{docstring Fin.reduceNatOp}
+
+{docstring Fin.reduceNatAdd}
+
+{docstring Fin.reduceAddNat}
+
+{docstring Fin.reduceSub}
+
+{docstring Fin.reduceSubNat}
+
+{docstring Fin.reduceMul}
+
+{docstring Fin.reduceDiv}
+
+{docstring Fin.reduceMod}
+
+{docstring Fin.reduceBin}
+
+{docstring Fin.reducePred}
+
+{docstring Fin.reduceBinPred}
+
+{docstring Fin.reduceBoolPred}
+
+{docstring Fin.reduceBNe}
+
+{docstring Fin.reduceEq}
+
+{docstring Fin.reduceLT}
+
+{docstring Fin.reduceGE}
+
+{docstring Fin.reduceGT}
+
+{docstring Fin.reduceLE}
+
+{docstring Fin.reduceNe}
+
+{docstring Fin.reduceBEq}
+
+{docstring Fin.reduceRev}
+
+{docstring Fin.reduceFinMk}
+
+{docstring Fin.reduceXor}
+
+{docstring Fin.reduceOp}
+
+{docstring Fin.reduceAnd}
+
+{docstring Fin.reduceOr}
+
+{docstring Fin.reduceLast}
+
+{docstring Fin.reduceShiftLeft}
+
+{docstring Fin.reduceShiftRight}
+
+{docstring Fin.reduceCastSucc}
+
+{docstring Fin.reduceCastAdd}
+
+{docstring Fin.reduceCastLT}
+
+{docstring Fin.reduceCastLE}
